src/Crypto/Signature.dfy
@@ -6,48 +6,42 @@ module {:extern "Signature"} Signature {
     import opened StandardLibrary
     import opened UInt = StandardLibrary.UInt
 
-    datatype {:extern "Msg"} Msg = Msg(m: seq<uint8>)
-    datatype {:extern "SigningKey"} SigningKey = SK(k : seq<uint8>)
-    datatype {:extern "VerifKey"} VerifKey = VK(k : seq<uint8>)
-    datatype {:extern "Sig"} Sig = Sig(c : seq<uint8>)
+    datatype {:extern "ECDSAParams"} ECDSAParams = ECDSA_P384 | ECDSA_P256
 
-    datatype ECDSAParams = ECDSA_P384 | ECDSA_P256
+    // TODO: I keep signatures as pairs (r,s) for now until I understand how they are encoded in the message header
+    type Sig = (seq<uint8>, seq<uint8>)
 
-    function method MaxMsgLen (s : ECDSAParams) : Option<nat> { None }
-    function method VKLen (s : ECDSAParams) : nat { 0 }
-    predicate WfSig (s : ECDSAParams, sig : Sig) { true }
-    predicate WfSK (s : ECDSAParams, sk : SigningKey) { true }
-    predicate WfVK (s : ECDSAParams, vk : VerifKey) { |vk.k| == VKLen(s) && true }
-    predicate IsSignKeypair (s : ECDSAParams, sk : SigningKey, vk : VerifKey) { true }
+    class {:extern "ECDSA"} ECDSA {
 
-    function method VKOfSK (s : ECDSAParams, sk : SigningKey) : (vk : VerifKey)
-        requires WfSK(s, sk)
-        ensures WfVK(s, vk)
-        ensures IsSignKeypair(s, sk, vk) {
-            VK([])
-        }
+//        static function method MaxMsgLen (s : ECDSAParams) : Option<nat> { None }
 
-    method KeyGen(s : ECDSAParams) returns (sk : SigningKey, vk : VerifKey)
-        ensures WfSK(s, sk)
-        ensures WfVK(s, vk)
-        ensures IsSignKeypair(s, sk, vk)
-        ensures VKOfSK(s, sk) == vk {
-            sk := SK([]);
-            vk := VK([]);
-        }
+        static predicate {:axiom} WfSig (s : ECDSAParams, sig : Sig)
+        static predicate {:axiom} WfSK (s : ECDSAParams, sk : seq<uint8>) 
+        static predicate {:axiom} WfVK (s : ECDSAParams, vk : seq<uint8>) 
+        static predicate {:axiom} IsSignKeypair (s : ECDSAParams, sk : seq<uint8>, vk : seq<uint8>) 
 
-    function method Verify(s : ECDSAParams, vk : VerifKey, m : Msg, sig : Sig) : bool
-        requires WfVK(s, vk)
-        requires MaxMsgLen(s).Some? ==> |m.m| <= MaxMsgLen(s).get
-        requires WfSig(s, sig) {
-            true
-        }
+        /*
+        static function method VKOfSK (s : ECDSAParams, sk : seq<uint8>) : (vk : seq<uint8>)
+            requires WfSK(s, sk)
+            ensures WfVK(s, vk)
+            ensures IsSignKeypair(s, sk, vk) 
+            */
 
-    method Sign(s : ECDSAParams, sk : SigningKey, m : Msg) returns (sig : Option<Sig>)
-        requires WfSK(s, sk)
-        requires MaxMsgLen(s).Some? ==> |m.m| <= MaxMsgLen(s).get
-        ensures sig.Some? ==> WfSig(s, sig.get)
-        ensures sig.Some? ==> forall vk :: WfVK(s, vk) ==> IsSignKeypair(s, sk, vk) ==> Verify(s, vk, m, sig.get) == true {
+        static method {:extern "KeyGen"} KeyGen(s : ECDSAParams) returns (res : Option<(seq<uint8>, seq<uint8>)>)
+            ensures res.Some? ==> WfSK(s, res.get.1)
+            ensures res.Some? ==> WfVK(s, res.get.0)
+            ensures res.Some? ==> IsSignKeypair(s, res.get.1, res.get.0)
+//            ensures VKOfSK(s, sk) == vk 
 
-        }
+        static function method {:extern "Verify"} Verify(s : ECDSAParams, vk : seq<uint8>, m : seq<uint8>, sig : Sig) : bool
+            requires WfVK(s, vk)
+ //           requires MaxMsgLen(s).Some? ==> |m| <= MaxMsgLen(s).get
+            requires WfSig(s, sig)
+
+        static method {:extern "Sign"} Sign(s : ECDSAParams, sk : seq<uint8>, m : seq<uint8>) returns (sig : Option<Sig>)
+            requires WfSK(s, sk)
+  //          requires MaxMsgLen(s).Some? ==> |m| <= MaxMsgLen(s).get
+            ensures sig.Some? ==> WfSig(s, sig.get)
+            ensures sig.Some? ==> forall vk :: WfVK(s, vk) ==> IsSignKeypair(s, sk, vk) ==> Verify(s, vk, m, sig.get) == true 
+    }
 }
