src/SDK/Keyring/RSAKeyring.dfy
@@ -1,0 +1,113 @@
+include "../MessageHeader/Definitions.dfy"
+include "../../StandardLibrary/StandardLibrary.dfy"
+include "../../StandardLibrary/UInt.dfy"
+include "../AlgorithmSuite.dfy"
+include "./Defs.dfy"
+include "../../Crypto/Cipher.dfy"
+include "../../Crypto/GenBytes.dfy"
+include "../../Crypto/RSAEncryption.dfy"
+include "../Common.dfy"
+
+module RSAKeyringDef {
+    import opened KeyringDefs
+    import opened StandardLibrary
+    import opened UInt = StandardLibrary.UInt
+    import opened Cipher
+    import GenBytes = RNG
+    import AlgorithmSuite
+    import RSA = RSAEncryption
+    import opened SDKDefs
+
+    class RSAKeyring extends Keyring {
+        const key_namespace : seq<uint8>
+        const key_name : seq<uint8>
+        const rsa_params : (RSA.RSAPaddingMode, RSA.RSABitLength)
+        const enc_key : Option<seq<uint8>>
+        const dec_key : Option<seq<uint8>>
+
+        predicate Valid() reads this {
+            Repr == {this} &&
+            (enc_key.Some? ==> RSA.RSA.RSAWfEK(rsa_params.1, rsa_params.0, enc_key.get)) &&
+            (dec_key.Some? ==> RSA.RSA.RSAWfDK(rsa_params.1, rsa_params.0, dec_key.get)) &&
+            (enc_key.Some? || dec_key.Some?)
+        }
+
+        constructor(namespace : seq<uint8>, name : seq<uint8>, padding : RSA.RSAPaddingMode, bits : RSA.RSABitLength, ek: Option<seq<uint8>>, dk: Option<seq<uint8>>)
+            requires ek.Some? ==> RSA.RSA.RSAWfEK(bits, padding, ek.get)
+            requires dk.Some? ==> RSA.RSA.RSAWfDK(bits, padding, dk.get)
+            requires (ek.Some? || dk.Some?)
+            ensures key_namespace == namespace
+            ensures key_name == name
+            ensures rsa_params == (padding, bits)
+            ensures enc_key == ek
+            ensures dec_key == dk
+            ensures Valid()
+        {
+            key_namespace := namespace;
+            key_name := name;
+            rsa_params := (padding, bits);
+            enc_key := ek;
+            dec_key := dk;
+            Repr := {this};
+        }
+
+        method OnEncrypt(x : EncMaterials) returns (res : Result<EncMaterials>)
+            requires WFEncMaterials(x)
+            requires Valid() ensures Valid()
+            ensures res.Ok? ==> WFEncMaterials(res.get)
+            ensures res.Ok? ==> res.get.alg_id == x.alg_id
+            ensures enc_key.None? ==> res.Err?
+        {
+            if enc_key.None? {
+                res := Err("Encryption key undefined");
+            }
+            else {
+                var data_key := x.data_key;
+                var alg_id := x.alg_id;
+                if data_key.None? {
+                    var k := RNG.GenBytes(AlgorithmSuite.input_key_length(alg_id) as uint16);
+                    data_key := Some(k);
+                }
+                var aad := FlattenSortEncCtx(x.enc_ctx);
+                var edk_ctxt := RSA.RSA.RSAEncrypt(rsa_params.1, rsa_params.0, enc_key.get, data_key.get);
+                if edk_ctxt.None? { return Err("Error on encrypt!"); }
+                var provider_id := key_namespace;
+                var provider_info := key_name;
+                return Ok(EncMat((alg_id), [EDK(provider_id, provider_info, edk_ctxt.get)] + x.edks, x.enc_ctx, data_key, None));
+
+            }
+
+        }
+
+
+        method OnDecrypt(x : DecMaterials, edks : seq<EDK>) returns (res : Result<DecMaterials>)
+            requires Valid() 
+            requires WFDecMaterials(x)
+            ensures Valid()
+            ensures res.Ok? ==> WFDecMaterials(res.get)
+            ensures res.Ok? ==> res.get.alg_id == x.alg_id
+            ensures dec_key.None? ==> res.Err?
+        {
+            if dec_key.None? { return Err(("Decryption key undefined"));}
+            if |edks| == 0 { return Err(("Ran out of edks")); }
+            if edks[0].provider_id != key_namespace { var x := OnDecrypt(x, edks[1..]); return x;}
+            if edks[0].provider_info != key_name { var x := OnDecrypt(x, edks[1..]); return x;}
+            var octxt := RSA.RSA.RSADecrypt(rsa_params.1, rsa_params.0, dec_key.get, edks[0].ciphertext);
+            match octxt {
+                    case None => {var x := OnDecrypt(x, edks[1..]); return x;}
+                    case Some(k) => {
+                            if |k| == AlgorithmSuite.input_key_length(x.alg_id) { // check for correct key length
+                                return Ok(DecMat(x.alg_id, x.enc_ctx, Some(k), None));
+                            }
+                            else {
+                                return Err(("Bad key length!"));
+                            }
+                    }
+
+            }
+        }
+
+
+    }
+
+}
